some tidying up

src/lib/kuiper/Kuiper.Divides.fst
@@ -3,6 +3,11 @@ module Kuiper.Divides
 open FStar.Mul
 module M = FStar.Math.Lemmas
 
+let get_factor (x y : int)
+  : Ghost int (requires x /? y)
+              (ensures fun z -> x * z == y)
+  = FStar.IndefiniteDescription.indefinite_description_ghost int (fun z -> x * z == y)
+
 let lemma_divides_mod1 (x:pos) (y:int)
   : Lemma (x /? y ==> y % x == 0)
 = let aux (z:int) : Lemma (requires z * x == y) (ensures y % x == 0) =
@@ -31,7 +36,6 @@ let lemma_divides_mod (x:pos) (y : int)
   Classical.forall_intro_2 aux;
   ()
 
-(* add reciprocal too? *)
 let lemma_divides_exact (x:pos) (y:int)
   : Lemma (x /? y <==> x * (y/x) == y)
 = lemma_divides_mod1 x y;
@@ -42,3 +46,23 @@ let lemma_divides_le (x : nat) (y : pos)
           (ensures x <= y)
           [SMTPat (x /? y)]
 = ()
+
+let lemma_divides_trans (x y z : pos)
+  : Lemma (requires x /? y /\ y /? z)
+          (ensures x /? z)
+          [SMTPat (x /? y); SMTPat (y /? z)]
+  = let f1 = get_factor x y in
+    let f2 = get_factor y z in
+    assert (x * (f1*f2) == z);
+    ()
+
+let rec lemma_pow2_div (x y : nat)
+  : Lemma (requires x <= y)
+          (ensures pow2 x /? pow2 y)
+          (decreases (y-x))
+          [SMTPat (pow2 x /? pow2 y)]
+= if x = y then ()
+  else (
+    lemma_pow2_div (x+1) y;
+    lemma_divides_trans (pow2 x) (pow2 (x+1)) (pow2 y)
+  )
