src/lib/kuiper/Kuiper.Divides.fsti
@@ -8,6 +8,10 @@ let divides (x y : int) : prop =
 unfold
 let ( /? ) = divides
 
+val get_factor (x y : int)
+  : Ghost int (requires x /? y)
+              (ensures fun z -> x * z == y)
+
 val lemma_divides_mod (x:pos) (y : int)
   : Lemma (x /? y <==> y % x == 0)
           [SMTPat (x /? y)]
@@ -20,3 +24,13 @@ val lemma_divides_le (x : nat) (y : pos)
   : Lemma (requires x /? y)
           (ensures x <= y)
           [SMTPat (x /? y)]
+
+val lemma_divides_trans (x y z : pos)
+  : Lemma (requires x /? y /\ y /? z)
+          (ensures x /? z)
+          [SMTPat (x /? y); SMTPat (y /? z)]
+
+val lemma_pow2_div (x y : nat)
+  : Lemma (requires x <= y)
+          (ensures pow2 x /? pow2 y)
+          [SMTPat (pow2 x /? pow2 y)]
