src/lib/kuiper/Kuiper.Math.fst
@@ -43,19 +43,17 @@ let lemma_log2_le2 (n:pos) (m:nat) : Lemma (n <= pow2 m ==> log2 n <= m) =
     log2 n <= m <: prop;
   }
 
-let rec div_pow2_lemma (i j tid: nat):
+let div_pow2_lemma (i j tid: nat) :
   Lemma
     (requires i < j)
     (ensures (div_pow2 j tid) ==> (div_pow2 i tid))
-  = if not (div_pow2 j tid) then () else (
-      if i = j - 1 then () else div_pow2_lemma i (j - 1) tid;
-      M.mod_mult_exact tid (pow2 (j - 1)) 2
-  )
+  = assert (pow2 i /? pow2 j) // from lemma_pow2_div and lemma_divides_trans, nice
 
 val lemma_div_exact: a:int -> p:pos -> Lemma
   (a % p = 0 <==> a = p * (a / p))
 let lemma_div_exact a p = ()
 
+#push-options "--z3rlimit 20"
 let div_pow2_lemma_2 (it tid: nat):
   Lemma (
     (not (div_pow2 (it + 1) (tid + pow2 it)) && div_pow2 it (tid + pow2 it))
@@ -83,7 +81,7 @@ let div_pow2_lemma_2 (it tid: nat):
       <==> { div_pow2_lemma it (it + 1) tid }
       div_pow2 (it + 1) tid;
     }
-
+#pop-options
 
 let shift_left_1_n (n:pos) (s:nat{s < n}) :
   Lemma (UInt.shift_left #n 1 s == pow2 s) =
